More examples.

theories/examples.v
@@ -64,13 +64,18 @@ Definition example3 :=
   let idA := EApp (EVar "id") (EConstant "A") in
   EPair idA idA.
 
-
 Definition texan {A} (m : free A) (φ : A → Prop) :=
   ∀ (φ' : A → Prop),
   (∀ v, φ v → φ' v) →
   safe m φ'.
 
-Goal
+Ltac prove_texan :=
+  unfold texan;
+  let φ' := fresh "φ'" in
+  let finished := fresh "finished" in
+  intros φ' finished.
+
+Lemma spec_example3:
   ∀ (id : val),
   (∀ v, texan (call id v) (λ v', v' = v)) →
   let env := EnvCons "id" id EnvNil in
@@ -83,4 +88,56 @@ Proof.
   apply Hid. intros v ?. subst v.
   wp.
   reflexivity.
+Qed.
+
+(* The identity function. *)
+
+(* [identity] is an expression which returns a closure whose behavior is
+   the identity function. *)
+
+Definition identity :=
+  ERec "self" "x" (EVar "x").
+
+Lemma spec_identity:
+  wp EnvNil identity (λ c, ∀ v, texan (call c v) (λ v', v' = v)).
+Proof.
+  wp. intros c.
+  prove_texan.
+  wp. eauto.
+Qed.
+
+(* let id = identity in
+   (id (A()), id (A())) *)
+
+Definition example4 :=
+  ELet (PVar "id") identity $
+  example3.
+
+Goal
+  wp EnvNil example4 (λ v, v = VPair (VConstant "A") (VConstant "A")).
+Proof.
+  (* This goes too far! I was expecting to re-use the specs that were proved
+     earlier about [example3] and [identity], but the interpreter executes
+     the whole program. The next example shows how to avoid this problem. *)
+  wp. reflexivity.
+Qed.
+
+Ltac wp_use H :=
+  eapply safe_covariant; [| eapply H ].
+
+Lemma spec_example4:
+  wp EnvNil example4 (λ v, v = VPair (VConstant "A") (VConstant "A")).
+Proof.
+  unfold example4.
+  (* Abstract away the [identity] function; its spec suffices. *)
+  generalize identity spec_identity.
+  intros identity Hidentity.
+  (* Abstract away [example3]; its spec suffices. *)
+  generalize example3 spec_example3.
+  intros example3 Hexample3.
+  (* Attack the goal. *)
+  wp.
+  wp_use Hidentity. simpl. intros id Hid.
+  wp_use (Hexample3 _ Hid).
+  simpl. eauto.
 Qed.
